Add more stuff to Imp.v

theories/Imp.v
@@ -1,17 +1,31 @@
 Set Implicit Arguments.
 Unset Strict Implicit.
 Unset Printing Implicit Defensive.
-From Coq Require Import ssreflect.
+From mathcomp Require Import ssreflect ssrnat.
 
+Require Import Coq.Strings.String.
+Require Import Nat.
 Require Import Maps.
+
+Definition state := total_map nat.
+
+Definition empty_state : state := t_empty 0.
+
+Notation "[<>]" := empty_state (at level 30) : type_scope.
+
+Definition W : string := "W".
+Definition X : string := "X".
+Definition Y : string := "Y".
+Definition Z : string := "Z".
 
 Inductive aexp : Type :=
 (* | AAny : aexp *)
 | ANum : nat -> aexp
+| AId : string -> aexp
 | APlus : aexp -> aexp -> aexp
 | AMinus : aexp -> aexp -> aexp
-| AMult : aexp -> aexp -> aexp
-| ADiv : aexp -> aexp -> aexp.
+| AMult : aexp -> aexp -> aexp.
+(* | ADiv : aexp -> aexp -> aexp. *)
 
 Reserved Notation "t ==> t'" (at level 50).
 
@@ -26,9 +40,202 @@ Inductive aevalR : aexp -> nat -> Prop :=
     (a1 ==> n1) -> (a2 ==> n2) -> (AMinus a1 a2) ==> (n1 - n2)
 | E_AMult : forall (a1 a2 : aexp) (n1 n2 : nat),
     (a1 ==> n1) -> (a2 ==> n2) -> (AMult a1 a2) ==> (n1 * n2)
-| E_ADiv : forall (a1 a2 : aexp) (n1 n2 n3 : nat),
-    (a1 ==> n1) -> (a2 ==> n2) -> (n2 > 0) ->
-    (mult n2 n3 = n1) -> (ADiv a1 a2) ==> n3
+(* | E_ADiv : forall (a1 a2 : aexp) (n1 n2 n3 : nat), *)
+(*     (a1 ==> n1) -> (a2 ==> n2) -> (n2 > 0) -> *)
+(*     (mult n2 n3 = n1) -> (ADiv a1 a2) ==> n3 *)
 where "a ==> n" := (aevalR a n).
 
-Definition state := total_map nat.
+Inductive bexp : Type :=
+| BTrue : bexp
+| BFalse : bexp
+| BEq : aexp -> aexp -> bexp
+| BLe : aexp -> aexp -> bexp
+| BNot : bexp -> bexp
+| BAnd : bexp -> bexp -> bexp.
+
+Coercion AId : string >-> aexp.
+Coercion ANum : nat >-> aexp.
+
+Definition bool_to_bexp (b : bool) : bexp :=
+  if b then BTrue else BFalse.
+
+Coercion bool_to_bexp : bool >-> bexp.
+
+Bind Scope aexp_scope with aexp.
+
+Infix "+" := APlus : aexp_scope.
+Infix "-" := AMinus : aexp_scope.
+Infix "*" := AMult : aexp_scope.
+
+Bind Scope bexp_scope with bexp.
+
+Notation "a '<.=' b" := (BLe a b) (at level 60) : bexp_scope.
+Notation "a '=.=' b" := (BEq a b) (at level 60) : bexp_scope.
+Notation "a '&.&' b" := (BAnd a b) (at level 60) : bexp_scope.
+Notation "'!' b" := (BNot b) (at level 60) : bexp_scope.
+
+Fixpoint aeval (st : state) (a : aexp) : nat :=
+  match a with
+  | ANum n => n
+  | AId x => st x
+  | APlus a1 a2 => (aeval st a1) + (aeval st a2)
+  | AMinus a1 a2 => (aeval st a1) - (aeval st a2)
+  | AMult a1 a2 => (aeval st a1) * (aeval st a2)
+  end.
+
+Fixpoint beval (st : state) (b : bexp) : bool :=
+  match b with
+  | BTrue => true
+  | BFalse => false
+  | BEq a1 a2 => eqn (aeval st a1) (aeval st a2)
+  | BLe a1 a2 => leb (aeval st a1) (aeval st a2)
+  | BNot b1 => negb (beval st b1)
+  | BAnd b1 b2 => andb (beval st b1) (beval st b2)
+  end.
+
+Example aexp1 :
+  aeval ([<>] [<X ~~>> 5>]) (3 + (X * 2)) = 13.
+Proof. by []. Qed.
+
+Example bexp1 :
+  beval ([<>] [<X ~~>> 5>]) (true &.& !(X <.= 4)) = true.
+Proof. by []. Qed.
+
+Inductive com : Type :=
+| CSkip : com
+| CAss : string -> aexp -> com
+| CSeq : com -> com -> com
+| CIf : bexp -> com -> com -> com
+| CWhile : bexp -> com -> com.
+
+Notation "'SKIP'" :=
+  CSkip.
+Notation "x '::=' a" :=
+  (CAss x a) (at level 60).
+Notation "c1 ;; c2" :=
+  (CSeq c1 c2) (at level 80, right associativity).
+Notation "'WHILE' b 'DO' c 'END'" :=
+  (CWhile b c) (at level 80, right associativity).
+Notation "'IFB' c1 'THEN' c2 'ELSE' c3 'FI'" :=
+  (CIf c1 c2 c3) (at level 80, right associativity).
+
+Definition fact_in_coq : com :=
+  Z ::= X;;
+  Y ::= 1;;
+  WHILE !(Z =.= 0) DO
+    Y ::= Y * Z;;
+    Z ::= Z - 1
+  END.
+
+Definition plus2 : com :=
+  X ::= X + 2.
+
+Definition XtimesYinZ : com :=
+  Z ::= X * Y.
+
+Definition subtract_slowly_body : com :=
+  Z ::= Z - 1;;
+  X ::= X - 1.
+
+Definition subtract_slowly : com :=
+  WHILE !(X =.= 0) DO
+    subtract_slowly_body
+  END.
+
+Definition subtract_3_from_5_slowly : com :=
+  X ::= 3;;
+  Z ::= 5;;
+  subtract_slowly.
+
+Definition loop : com :=
+  WHILE BTrue DO
+    SKIP
+  END.
+
+Definition exp_body : com :=
+  Z ::= Z * X;;
+  Y ::= Y - 1.
+
+Definition pexp : com :=
+  WHILE !(Y =.= 0) DO
+    exp_body
+  END.
+
+Reserved Notation "c1 '/' st '==>' st'"
+         (at level 40, st at level 39).
+
+Inductive ceval : com -> state -> state -> Prop :=
+| E_Skip : forall st,
+    SKIP / st ==> st
+| E_Ass : forall st a1 v k,
+    aeval st a1 = v ->
+    (k ::= a1) / st ==> st [< k ~~>> v >]
+| E_Seq : forall c1 c2 st st' st'',
+    c1 / st  ==> st'  ->
+    c2 / st' ==> st'' ->
+    (c1 ;; c2) / st ==> st''
+| E_IfTrue : forall st st' b c1 c2,
+    beval st b = true ->
+    c1 / st ==> st' ->
+    (IFB b THEN c1 ELSE c2 FI) / st ==> st'
+| E_IfFalse : forall st st' b c1 c2,
+    beval st b = false ->
+    c2 / st ==> st' ->
+    (IFB b THEN c1 ELSE c2 FI) / st ==> st'
+| E_WhileEnd : forall b st c,
+    beval st b = false ->
+    (WHILE b DO c END) / st ==> st
+| E_WhileLoop : forall st st' st'' b c,
+    beval st b = true ->
+    c / st ==> st' ->
+    (WHILE b DO c END) / st' ==> st'' ->
+    (WHILE b DO c END) / st  ==> st''
+
+where "c1 '/' st '==>' st'" := (ceval c1 st st').
+
+Inductive cevalR (c : com) (st st' : state) : Prop :=
+  | E_Skip' of (c = SKIP) & (st = st')
+  | E_Ass' : forall a1 v k,
+      aeval st a1 = v ->
+      c = (k ::= a1) ->
+      st' = (st [< k ~~>> v >]) ->
+      cevalR c st st'
+  | E_Seq' : forall c1 c2 st'',
+      cevalR c1 st st'' ->
+      cevalR c2 st'' st' ->
+      c = (c1 ;; c2) ->
+      cevalR c st st'
+  | E_IfTrue' : forall b c1 c2,
+      beval st b = true ->
+      cevalR c1 st st' ->
+      c = (IFB b THEN c1 ELSE c2 FI) ->
+      cevalR c st st'
+  | E_IfFalse' : forall b c1 c2,
+      beval st b = false ->
+      cevalR c2 st st' ->
+      c = (IFB b THEN c1 ELSE c2 FI) ->
+      cevalR c st st'
+  | E_WhileEnd' : forall b d,
+      beval st b = false ->
+      c = (WHILE b DO d END) ->
+      st' = st ->
+      cevalR c st st'
+  | E_WhileLoop' : forall st'' b d,
+      beval st b = true ->
+      cevalR d st st'' ->
+      cevalR c st'' st' ->
+      c = (WHILE b DO d END) ->
+      cevalR c st st'.
+
+Example ceval_example1 :
+  (X ::= 2;;
+   IFB X <.= 1
+     THEN Y ::= 3
+     ELSE Z ::= 4
+   FI)
+  / [<>]
+  ==> [<>] [<X ~~>> 2>] [<Z ~~>> 4>].
+Proof.
+  apply: E_Seq.
+  Unshelve.
+Qed.
